src/hmem/encoding/list_complexity.lean
@@ -1,0 +1,332 @@
+import hmem.stack
+import hmem.encoding.list
+import hmem.split_cost
+import complexity.basic
+
+variables {μ: Type*} [decidable_eq μ] [has_zero μ] [has_one μ] [ne_zero (1:μ)]
+
+namespace hmem
+namespace encoding
+
+theorem split_complexity {α: Type*} [complexity.has_encoding (runtime_model μ) α] (l: list α):
+  (split μ).has_time_cost (encode l) (5 * l.length + 3) :=
+begin
+  induction l,
+  { apply thunk.time_cost_of_split',
+    apply thunk.has_trace.split_cost,
+    apply split_has_trace,
+    apply list.sum_le_nil,
+    apply list.sum_le_nil,
+    simp only [list.length, split_trace, mul_zero, add_zero] },
+  { apply thunk.time_cost_of_split',
+    apply thunk.has_trace.split_cost,
+    apply split_has_trace,
+    apply list.sum_le_nil,
+    apply list.sum_le_cons l_ih list.sum_le_nil,
+    unfold split_trace list.length,
+    ring }
+end
+
+theorem merge_complexity {α: Type*} [complexity.has_encoding (runtime_model μ) α]
+  (fcmp: α → α → Prop) [dcmp: decidable_rel fcmp]
+  {pcmp: program μ} (hcmp: ∀ (a b: α), pcmp.has_result (encode (a, b)) (encode (dcmp a b)))
+  {c: ℕ}
+  {as bs: list α}
+  (hcost: ∀ a b, a ∈ as → b ∈ bs → pcmp.has_time_cost (encode (a, b)) c):
+  (merge pcmp).has_time_cost (encode (as, bs)) ((19 + c) * (as.length + bs.length) + 4) :=
+begin
+  induction h:(as.length + bs.length) using nat.strong_induction_on with n ih generalizing as bs,
+  cases as with a as,
+  { apply program.time_cost_mono,
+    apply thunk.time_cost_of_split',
+    apply thunk.has_trace.split_cost,
+    apply merge_has_trace fcmp hcmp,
+    apply list.sum_le_nil,
+    apply list.sum_le_nil,
+    unfold merge_trace,
+    ring_nf,
+    apply le_add_left,
+    apply le_add_left,
+    apply le_refl, },
+  cases bs with b bs,
+  { apply program.time_cost_mono,
+    apply thunk.time_cost_of_split',
+    apply thunk.has_trace.split_cost,
+    apply merge_has_trace fcmp hcmp,
+    apply list.sum_le_nil,
+    apply list.sum_le_nil,
+    unfold merge_trace,
+    rw [← h],
+    unfold list.length,
+    ring_nf,
+    apply le_add_left,
+    linarith },
+  by_cases hab:fcmp a b,
+  { apply program.time_cost_mono,
+    apply thunk.time_cost_of_split',
+    apply thunk.has_trace.split_cost,
+    apply merge_has_trace fcmp hcmp,
+    { simp only [merge_trace, hab, if_true],
+      apply list.sum_le_cons,
+      apply hcost,
+      apply list.mem_cons_self,
+      apply list.mem_cons_self,
+      apply list.sum_le_nil },
+    { simp only [merge_trace, hab, if_true],
+      apply list.sum_le_cons,
+      apply ih _ _ _ rfl,
+      simpa only [← h, list.length, ← add_assoc, add_lt_add_iff_right] using nat.lt_succ_self _,
+      { intros a b ha hb,
+        apply hcost _ _ _ hb,
+        apply list.mem_cons_of_mem _ ha },
+      apply list.sum_le_nil },
+    refl,
+    simp only [hab, if_true, ← h, list.length, merge_trace, list.length],
+    linarith },
+  { apply program.time_cost_mono,
+    apply thunk.time_cost_of_split',
+    apply thunk.has_trace.split_cost,
+    apply merge_has_trace fcmp hcmp,
+    { simp only [merge_trace, hab, if_false],
+      apply list.sum_le_cons,
+      apply hcost,
+      apply list.mem_cons_self,
+      apply list.mem_cons_self,
+      apply list.sum_le_nil },
+    { simp only [merge_trace, hab, if_false],
+      apply list.sum_le_cons,
+      apply ih _ _ _ rfl,
+      simpa only [← h, list.length, ← add_assoc, add_lt_add_iff_right] using nat.lt_succ_self _,
+      { intros a b ha hb,
+        apply hcost _ _ ha,
+        apply list.mem_cons_of_mem _ hb },
+      apply list.sum_le_nil },
+    refl,
+    simp only [hab, if_false, ← h, list.length, merge_trace, list.length],
+    linarith },
+end
+
+
+-- def merge_trace {α: Type*} [complexity.has_encoding (runtime_model μ) α] (fcmp: α → α → Prop) [dcmp: decidable_rel fcmp] (pcmp: program μ):
+--   list α → list α → trace μ
+-- | [] b := ⟨ encode b, 3, [], [] ⟩
+-- | (a::as) [] := ⟨ encode (a::as), 5, [], [] ⟩
+-- | (a::as) (b::bs) := if (fcmp a b)
+--   then ⟨ encode (list.merge fcmp (a::as) (b::bs)), 16, [(pcmp, (encode (a, b)))], [encode (as, b::bs)] ⟩
+--   else ⟨ encode (list.merge fcmp (a::as) (b::bs)), 18, [(pcmp, (encode (a, b)))], [encode (a::as, bs)] ⟩
+
+-- f(0) = 3
+-- f(1) = 5
+-- f(n) = 13 + (24 + c) * n  + 2 * f (n / 2)
+-- f(2) = 83 + c * 2
+-- f(4) = 287 + c * 8
+-- f(8) = 791 + c * 16
+
+-- f(0) = 0
+-- f(1) = 0
+-- f(n) = c * n  + 2 * f (n / 2)
+-- f(2) = 2c
+-- f(4) = 8c
+-- f(8) = 24c
+-- f(16) = 64c
+
+theorem list.perm_split {α: Type*} : ∀ (l : list α), l ~ l.split.fst ++ l.split.snd
+| [] := by simp
+| (a::l) :=
+begin
+  unfold list.split,
+  cases h:l.split,
+  unfold list.split,
+  simp,
+  refine (list.perm_split _).trans _,
+  simp [h],
+  exact list.perm_append_comm,
+end
+
+theorem list.perm_split'  {α: Type*} {l l₀ l₁: list α}:
+  l.split = (l₀, l₁) → l ~ l₀ ++ l₁ :=
+begin
+  intro heq,
+  have h := list.perm_split l,
+  rw [heq] at h,
+  apply h,
+end
+
+theorem list.length_split {α: Type*} (l: list α):
+  l.split.fst.length = (l.length + 1) / 2 ∧ l.split.snd.length = l.length / 2 :=
+begin
+  induction l,
+  { simp [nat.div_eq_zero] },
+  cases h:l_tl.split,
+  simpa [h, nat.add_assoc, nat.succ_eq_add_one] using and.symm l_ih,
+end
+
+theorem list.length_split' {α: Type*} {l l₀ l₁: list α}:
+  l.split = (l₀, l₁) → l₀.length = (l.length + 1) / 2 ∧ l₁.length = l.length / 2 :=
+begin
+  intro heq,
+  have h := list.length_split l,
+  rw [heq] at h,
+  apply h,
+end
+
+theorem list.length_split_le' {α: Type*} {l l₀ l₁: list α}:
+  l.split = (l₀, l₁) → l₁.length ≤ l₀.length :=
+begin
+  intro heq,
+  simp only [list.length_split' heq],
+  apply nat.div_le_div_right,
+  apply nat.le_succ,
+end
+
+-- | []       []        := by simp [merge]
+-- | []       (b :: l') := by simp [merge]
+-- | (a :: l) []        := by simp [merge]
+-- | (a :: l) (b :: l') := begin
+--   by_cases a ≼ b,
+--   { simpa [merge, h] using perm_merge _ _ },
+--   { suffices : b :: merge r (a :: l) l' ~ a :: (l ++ b :: l'), {simpa [merge, h]},
+--     exact ((perm_merge _ _).cons _).trans ((swap _ _ _).trans (perm_middle.symm.cons _)) }
+-- end
+
+theorem merge_sort_complexity {α: Type*} [complexity.has_encoding (runtime_model μ) α]
+  (fcmp: α → α → Prop) [dcmp: decidable_rel fcmp]
+  {pcmp: program μ} (hcmp: ∀ (a b: α), pcmp.has_result (encode (a, b)) (encode (dcmp a b)))
+  {c: ℕ} {l: list α}
+  (hcost: ∀ a b, a ∈ l → b ∈ l → pcmp.has_time_cost (encode (a, b)) c):
+  (merge_sort pcmp).has_time_cost (encode l) ((37 + c) * l.length * (nat.clog 2 l.length) + 5) :=
+begin
+  induction h:l.length using nat.strong_induction_on with n ih generalizing l,
+  cases hsplit:l.split with l₀ l₁,
+  cases l with a l,
+  { rw [← h, list.length, mul_zero, zero_mul, zero_add],
+    apply program.time_cost_mono,
+    apply thunk.time_cost_of_split',
+    apply thunk.has_trace.split_cost,
+    apply merge_sort_has_trace fcmp hcmp,
+    apply list.sum_le_nil,
+    apply list.sum_le_nil,
+    unfold merge_sort_trace,
+    linarith },
+  cases l with b l,
+  { rw [← h, list.length, list.length, zero_add, nat.clog_one_right, mul_zero, zero_add],
+    apply program.time_cost_mono,
+    apply thunk.time_cost_of_split',
+    apply thunk.has_trace.split_cost,
+    apply merge_sort_has_trace fcmp hcmp,
+    apply list.sum_le_nil,
+    apply list.sum_le_nil,
+    unfold merge_sort_trace,
+    linarith },
+  apply program.time_cost_mono,
+  apply thunk.time_cost_of_split',
+  apply thunk.has_trace.split_cost,
+  apply merge_sort_has_trace fcmp hcmp,
+  { simp only [merge_sort_trace, hsplit],
+    apply list.sum_le_cons,
+    apply split_complexity,
+    apply list.sum_le_cons,
+    apply merge_complexity fcmp hcmp,
+    { intros a b ha hb,
+      apply hcost,
+      rw [list.perm.mem_iff (list.perm_merge_sort _ _)] at ha hb,
+      rw [list.perm.mem_iff (list.perm_split _), hsplit, list.mem_append],
+      exact or.inl ha,
+      rw [list.perm.mem_iff (list.perm_merge_sort _ _)] at ha hb,
+      rw [list.perm.mem_iff (list.perm_split _), hsplit, list.mem_append],
+      exact or.inr hb },
+    apply list.sum_le_nil },
+  { simp only [merge_sort_trace, hsplit],
+    apply list.sum_le_cons,
+    { apply ih _ _ _ rfl,
+      rw [← h],
+      apply (list.length_split_lt hsplit).left,
+      intros a b ha hb,
+      apply hcost,
+      rw [list.perm.mem_iff (list.perm_split _), hsplit, list.mem_append],
+      exact or.inl ha,
+      rw [list.perm.mem_iff (list.perm_split _), hsplit, list.mem_append],
+      exact or.inl hb },
+    apply list.sum_le_cons,
+    { apply ih _ _ _ rfl,
+      rw [← h],
+      apply (list.length_split_lt hsplit).right,
+      intros a b ha hb,
+      apply hcost,
+      rw [list.perm.mem_iff (list.perm_split _), hsplit, list.mem_append],
+      exact or.inr ha,
+      rw [list.perm.mem_iff (list.perm_split _), hsplit, list.mem_append],
+      exact or.inr hb },
+    exact list.sum_le_nil },
+  simp only [merge_sort_trace, hsplit],
+  ring_nf,
+  rw [nat.add_left_comm],
+  apply add_le_add,
+  { apply nat.mul_le_mul_right,
+    rw [← nat.add_assoc,
+      list.perm.length_eq (list.perm_merge_sort fcmp _),
+      list.perm.length_eq (list.perm_merge_sort fcmp _),
+      ← list.length_append, list.perm.length_eq (list.perm_split' hsplit).symm],
+    apply nat.le_trans,
+    { apply nat.add_le_add_left,
+      apply nat.add_le_add_left,
+      apply nat.mul_le_mul_right,
+      apply nat.clog_mono_right,
+      apply list.length_split_le' hsplit },
+    rw [← mul_add, ← list.length_append, list.perm.length_eq (list.perm_split' hsplit).symm, add_comm, ← nat.succ_mul, h],
+    apply nat.mul_le_mul_right,
+    rw [(list.length_split' hsplit).left, h,
+      show ∀ n : ℕ, n + 1 = n + 2 - 1,
+      begin
+          intro _,
+          simp [← nat.succ_eq_add_one],
+      end,
+      nat.succ_eq_add_one,
+      ← nat.clog_of_two_le (one_lt_two)],
+    rw [← h, list.length, list.length],
+    apply nat.succ_le_succ,
+    apply nat.succ_le_succ,
+    apply nat.zero_le },
+    rw [list.perm.length_eq (list.perm_merge_sort fcmp _), list.perm.length_eq (list.perm_merge_sort fcmp _),
+      show ∀ n m, (m * l₀.length + (m * l₁.length + n)) = m * (l₀.length + l₁.length) + n,
+      by simp only [nat.add_assoc, mul_add, eq_self_iff_true, forall_2_true_iff],
+      ← list.length_append, list.perm.length_eq (list.perm_split' hsplit).symm, h],
+    ring_nf,
+    apply nat.le_trans,
+    { apply add_le_add_left,
+      apply add_le_add_left,
+      apply add_le_add_right,
+      apply nat.mul_le_mul_left,
+      apply nat.clog_mono_right,
+      apply list.length_split_le' hsplit },
+    rw [mul_right_comm, mul_right_comm _ l₁.length,
+      show ∀ n m, (m * l₀.length + (m * l₁.length + n)) = m * (l₀.length + l₁.length) + n,
+      by simp only [nat.add_assoc, mul_add, eq_self_iff_true, forall_2_true_iff],
+      ← list.length_append, list.perm.length_eq (list.perm_split' hsplit).symm, h,
+      (list.length_split' hsplit).left, h,
+      show ∀ n : ℕ, n + 1 = n + 2 - 1,
+      begin
+          intro _,
+          simp [← nat.succ_eq_add_one],
+      end,
+      show ∀ n: ℕ, n + 2 - 1 = n + 1,
+      by simp only [← nat.succ_eq_add_one, ← nat.pred_eq_sub_one, nat.pred_succ, eq_self_iff_true, forall_true_iff]],
+    rw [← @nat.add_le_add_iff_right (13 * n)],
+    ring_nf,
+    rw [← nat.mul_succ, nat.succ_eq_add_one,
+      show n + 1 = n + 2 - 1,
+      by simp [← nat.succ_eq_add_one],
+      ← nat.clog_of_two_le (one_lt_two),
+      add_mul, nat.add_assoc],
+    apply add_le_add_left,
+    rw [← h, list.length, list.length],
+    linarith,
+    rw [← h, list.length, list.length],
+    apply nat.succ_le_succ,
+    apply nat.succ_le_succ,
+    apply zero_le _,
+end
+
+
+end encoding
+end hmem
