src/hmem/trace.lean
@@ -1,0 +1,341 @@
+import hmem.memory
+import hmem.split_cost
+import hmem.stack
+
+namespace hmem
+
+structure trace (α: Type*) [has_zero α] [decidable_eq α] :=
+  (result: memory α)
+  (steps: ℕ)
+  (calls: list (program α × memory α))
+  (recurses: list (memory α)) 
+
+universe u
+variables {α: Type u} [has_zero α] [decidable_eq α]
+
+def trace.has_call_cost (t: trace α) (c: ℕ): Prop :=
+  t.calls.sum_le (λ pm, pm.fst.has_time_cost pm.snd) c
+  
+def trace.has_recurse_cost (t: trace α) (p: program α) (r: ℕ): Prop :=
+  t.recurses.sum_le (λ m, p.has_time_cost m) r
+
+def thunk.extend_trace (t: thunk α): trace α → trace α
+| ⟨m, i, cs, rs⟩ := match t.step with
+  | (sum.inr (sum.inr (option.some p, m', _))) := ⟨m, i + 1, (p, m')::cs, rs⟩
+  | (sum.inr (sum.inr (option.none, m', _))) := ⟨m, i + 1, cs, m'::rs⟩
+  | _ := ⟨m, i + 1, cs, rs⟩
+end
+
+def thunk.extend_trace₀ {t t': thunk α} {tr: trace α} {m: memory α} {n: ℕ} {cs: list (program α × memory α)} {rs: list (memory α)}:
+  t.step = sum.inl t' → tr = ⟨m, n, cs, rs⟩ → t.extend_trace tr = ⟨m, n+1, cs, rs⟩ :=
+begin
+  intros hstep heq,
+  simp only [heq, thunk.extend_trace, hstep, eq_self_iff_true, and_true],
+end
+  
+
+theorem thunk.extend_trace_result (t : thunk α) (tr: trace α):
+  (t.extend_trace tr).result = tr.result :=
+begin
+  cases tr,
+  unfold thunk.extend_trace,
+  cases t.step,
+  { refl },
+  cases val,
+  { refl },
+  rcases val with ⟨_|_, _, _⟩;
+  refl,
+end
+
+theorem thunk.extend_trace_steps (t : thunk α) (tr: trace α):
+  (t.extend_trace tr).steps = tr.steps + 1 :=
+begin
+  cases tr,
+  unfold thunk.extend_trace,
+  cases t.step,
+  { refl },
+  cases val,
+  { refl },
+  rcases val with ⟨_|_, _, _⟩;
+  refl,
+end
+
+theorem thunk.extend_trace_calls_cons {t: thunk α} {tr: trace α} {p: program α} {t': thunk α} {m: memory α}:
+  t.step = sum.inr (sum.inr (some p, m, t')) → (t.extend_trace tr).calls = (p, m)::tr.calls :=
+begin
+  cases tr,
+  intro hstep,
+  simp only [thunk.extend_trace, hstep, eq_self_iff_true, and_true]
+end
+
+theorem thunk.extend_trace_calls_eq {t: thunk α} {tr: trace α}:
+  (∀ {p m t'}, t.step ≠ sum.inr (sum.inr (some p, m, t'))) → (t.extend_trace tr).calls = tr.calls :=
+begin
+  cases tr,
+  cases hstep: t.step,
+  { simp only [thunk.extend_trace, hstep, eq_self_iff_true, imp_true_iff] },
+  cases val,
+  { simp only [thunk.extend_trace, hstep, eq_self_iff_true, imp_true_iff] },
+  rcases val with ⟨_|_,_,_⟩,
+  { simp only [thunk.extend_trace, hstep, eq_self_iff_true, imp_true_iff] },
+  contrapose!,
+  simp,
+end
+
+theorem thunk.extend_trace_calls_eq₀ {t: thunk α} {tr: trace α} {t': thunk α}:
+  t.step = sum.inl t' → (t.extend_trace tr).calls = tr.calls :=
+begin
+  intro hstep,
+  apply thunk.extend_trace_calls_eq,
+  simp [hstep]
+end
+
+theorem thunk.extend_trace_calls_eq₁ {t: thunk α} {tr: trace α} {m: memory α}:
+  t.step = sum.inr (sum.inl m) → (t.extend_trace tr).calls = tr.calls :=
+begin
+  intro hstep,
+  apply thunk.extend_trace_calls_eq,
+  simp [hstep]
+end
+
+theorem thunk.extend_trace_calls_eq₂ {t: thunk α} {tr: trace α} {m: memory α} {t': thunk α}:
+  t.step = sum.inr (sum.inr (none, m, t')) → (t.extend_trace tr).calls = tr.calls :=
+begin
+  intro hstep,
+  apply thunk.extend_trace_calls_eq,
+  simp [hstep]
+end
+
+theorem thunk.extend_trace_recurses_cons {t: thunk α} {tr: trace α} {t': thunk α} {m: memory α}:
+  t.step = sum.inr (sum.inr (none, m, t')) → (t.extend_trace tr).recurses = m::tr.recurses :=
+begin
+  cases tr,
+  intro hstep,
+  simp only [thunk.extend_trace, hstep, eq_self_iff_true, and_true]
+end
+
+theorem thunk.extend_trace_recurses_eq {t: thunk α} {tr: trace α}:
+  (∀ {m t'}, t.step ≠ sum.inr (sum.inr (none, m, t'))) → (t.extend_trace tr).recurses = tr.recurses :=
+begin
+  cases tr,
+  cases hstep: t.step,
+  { simp only [thunk.extend_trace, hstep, eq_self_iff_true, imp_true_iff] },
+  cases val,
+  { simp only [thunk.extend_trace, hstep, eq_self_iff_true, imp_true_iff] },
+  rcases val with ⟨_|_,_,_⟩,
+  {contrapose!, simp },
+  { simp only [thunk.extend_trace, hstep, eq_self_iff_true, imp_true_iff] },
+end
+
+theorem thunk.extend_trace_recurses_eq₀ {t: thunk α} {tr: trace α} {t': thunk α}:
+  t.step = sum.inl t' → (t.extend_trace tr).recurses = tr.recurses :=
+begin
+  intro hstep,
+  apply thunk.extend_trace_recurses_eq,
+  simp [hstep]
+end
+
+theorem thunk.extend_trace_recurses_eq₁ {t: thunk α} {tr: trace α} {m: memory α}:
+  t.step = sum.inr (sum.inl m) → (t.extend_trace tr).recurses = tr.recurses :=
+begin
+  intro hstep,
+  apply thunk.extend_trace_recurses_eq,
+  simp [hstep]
+end
+
+theorem thunk.extend_trace_recurses_eq₂ {t: thunk α} {tr: trace α} {p: program α} {m: memory α} {t': thunk α}:
+  t.step = sum.inr (sum.inr (some p, m, t')) → (t.extend_trace tr).recurses = tr.recurses :=
+begin
+  intro hstep,
+  apply thunk.extend_trace_recurses_eq,
+  simp [hstep]
+end
+
+inductive thunk.has_trace: thunk α → trace α → Prop
+| result (p: program α) (m: memory α): thunk.has_trace ⟨p, [], m⟩ ⟨m, 0, [], []⟩
+| step {t t': thunk α} {tr: trace α} (ht: t.step_over t') (htr: thunk.has_trace t' tr):
+  thunk.has_trace t (thunk.extend_trace t tr)
+
+theorem thunk.has_trace_nil (t: thunk α) {tr: trace α}:
+  t.has_trace tr → t.current = [] → tr = ⟨t.state, 0, [], []⟩ :=
+begin
+  intros htr ht,
+  cases htr,
+  { refl },
+  cases t,
+  simp only [] at ht,
+  simpa [ht, thunk.step_over, thunk.step] using htr_ht,
+end
+theorem thunk.has_trace_result {t: thunk α} {tr: trace α}:
+  t.has_trace tr → (thunk.step_over^~[tr.steps]) t ⟨t.function, [], tr.result⟩ :=
+begin
+  intro htr,
+  induction htr,
+  { exact rel_iterate_zero _ _ },
+  rw [thunk.extend_trace_steps, thunk.extend_trace_result, rel_iterate_succ_iff, thunk.step_over_function htr_ht],
+  exact ⟨_, htr_ht, htr_ih⟩
+end
+
+theorem thunk.has_trace.exists_calls_sum {t: thunk α} {tr: trace α}:
+  t.has_trace tr → ∃ c, tr.has_call_cost c :=
+begin
+  unfold trace.has_call_cost,
+  intro htr,
+  induction htr,
+  { exact ⟨0, trivial⟩ },
+  cases hstep:htr_t.step,
+  { rwa [thunk.extend_trace_calls_eq₀ hstep] },
+  cases val,
+  { rwa [thunk.extend_trace_calls_eq₁ hstep] },
+  rcases val with ⟨_|_, _, _⟩,
+  { rwa [thunk.extend_trace_calls_eq₂ hstep] },
+  { simp only [thunk.step_over, option.get_or_else, option.map_some', hstep] at htr_ht,
+    cases htr_ht.left with c₀ hc₀,
+    cases htr_ih with c₁ hc₁,rw [thunk.extend_trace_calls_cons hstep],
+    exact ⟨_, _, _, ⟨_, hc₀⟩, hc₁, rfl⟩ }
+end
+
+theorem thunk.has_trace.exists_recurses_sum {t: thunk α} {tr: trace α}:
+  t.has_trace tr → ∃ r, tr.has_recurse_cost t.function r :=
+begin
+  unfold trace.has_recurse_cost,
+  intro htr,
+  induction htr,
+  { exact ⟨0, trivial⟩ },
+  cases hstep:htr_t.step,
+  { rwa [thunk.extend_trace_recurses_eq₀ hstep, thunk.step_over_function htr_ht] },
+  cases val,
+  { rwa [thunk.extend_trace_recurses_eq₁ hstep, thunk.step_over_function htr_ht] },
+  rcases val with ⟨_|_, _, _⟩,
+  { have hfunc := thunk.step_over_function htr_ht,
+    simp only [thunk.step_over, option.get_or_else, option.map_none', hstep] at htr_ht,
+    cases htr_ht.left with r₀ hr₀,
+    cases htr_ih with r₁ hr₁,
+    rw [thunk.extend_trace_recurses_cons hstep],
+    exact ⟨r₀ + r₁, r₀, r₁, ⟨_, hr₀⟩, hfunc.symm ▸ hr₁, rfl⟩ },
+  { rwa [thunk.extend_trace_recurses_eq₂ hstep, thunk.step_over_function htr_ht] },
+end
+
+theorem thunk.has_trace.split_cost {t: thunk α} {tr: trace α} {c r: ℕ}:
+  t.has_trace tr →
+  tr.has_call_cost c →
+  tr.has_recurse_cost t.function r →
+  t.split_time_cost (tr.steps + 1) c r :=
+begin
+  unfold trace.has_call_cost trace.has_recurse_cost,
+  intro htr,
+  induction htr generalizing c r,
+  { exact λ _ _, or.inl rfl },
+  cases hstep:htr_t.step,
+  { rw [thunk.extend_trace_calls_eq₀ hstep, thunk.extend_trace_recurses_eq₀ hstep, thunk.extend_trace_steps, thunk.step_over_function htr_ht],
+    intros hcs hrs,
+    refine or.inr ⟨_, _, _, _, _, _, htr_ht, _, (zero_add _).symm, (zero_add _).symm⟩,
+    { simp only [thunk.external_time_cost_step, hstep] },
+    exact htr_ih hcs hrs },
+  cases val,
+  { simpa only [thunk.step_over, thunk.step, hstep] using htr_ht },
+  rcases val with ⟨_ | _, _, _⟩,
+  { rw [thunk.extend_trace_calls_eq₂ hstep, thunk.extend_trace_recurses_cons hstep, thunk.extend_trace_steps, thunk.step_over_function htr_ht],
+    intros hcs hrs,
+    rcases hrs with ⟨r₀, r₁, hrcost, hrs, hr⟩,
+    refine or.inr ⟨_, _, _, _, _, _, htr_ht, _, (zero_add _).symm, hr⟩,
+    { simpa only [thunk.external_time_cost_step, hstep, option.map_none', option.get_or_else, thunk.step_over_function htr_ht] using hrcost },
+    exact htr_ih hcs hrs },
+  { rw [thunk.extend_trace_calls_cons hstep, thunk.extend_trace_recurses_eq₂ hstep, thunk.extend_trace_steps, thunk.step_over_function htr_ht],
+    intros hcs hrs,
+    rcases hcs with ⟨c₀, c₁, hccost, hcs, hc⟩,
+    refine or.inr ⟨_, _, _, _, _, _, htr_ht, _, hc, (zero_add _).symm⟩,
+    { simpa only [thunk.external_time_cost_step, hstep, option.map_some', option.get_or_else] using hccost },
+    exact htr_ih hcs hrs },
+end
+
+def program.has_trace (p: program α) (m: memory α) (t: trace α): Prop := thunk.has_trace ⟨p, p, m⟩ t
+
+theorem program.has_trace.result {p: program α} {m: memory α} {t: trace α}:
+  p.has_trace m t → p.has_result m t.result :=
+λ h, thunk.iterate_step_of_iterate_step_over' (thunk.has_trace_result h)
+
+theorem program.has_trace.internal_cost {p: program α} {m: memory α} {tr: trace α}:
+  p.has_trace m tr → p.internal_cost m (tr.steps + 1) :=
+begin
+  intros htr,
+  cases htr.exists_calls_sum with c hc,
+  cases htr.exists_recurses_sum with r hr,
+  exact ⟨_, _, htr.split_cost hc hr⟩
+end
+
+theorem program.has_trace.call_cost {p: program α} {m: memory α} {tr: trace α} {c: ℕ}:
+  p.has_trace m tr →
+  tr.has_call_cost c →
+  p.call_cost m c :=
+begin
+  intros htr hc,
+  cases htr.exists_recurses_sum with r hr,
+  exact ⟨_, _, htr.split_cost hc hr⟩
+end
+
+theorem program.has_trace.recurse_cost {p: program α} {m: memory α} {tr: trace α} {r: ℕ}:
+  p.has_trace m tr →
+  tr.has_recurse_cost p r →
+  p.recurse_cost m r :=
+begin
+  intros htr hr,
+  cases htr.exists_calls_sum with c hc,
+  exact ⟨_, _, htr.split_cost hc hr⟩
+end
+
+theorem start_trace {p is: program α} {inp: memory α} {tr: trace α}:
+  is = p →
+  thunk.has_trace ⟨p, is, inp⟩ tr →
+  p.has_trace inp tr :=
+λ h, h ▸ id
+
+theorem step_trace {t t': thunk α} {tr tr': trace α}:
+  t.step_over t' →
+  t.extend_trace tr' = tr →
+  t'.has_trace tr' →
+  t.has_trace tr :=
+λ hso hex htr, hex ▸ thunk.has_trace.step hso htr
+
+
+-- theorem apply_step_over_recurse {p: program α} {s: source α} {is: program α} {m m' r: memory α}:
+--   p.has_result (m.getms s) m' →
+--   (∃ n, (stack.step^[n]) (stack.execution ⟨p, is, m.setm 0 m'⟩ []) = stack.result r) →
+--   (∃ n, (stack.step^[n]) (stack.execution ⟨p, (instruction.recurse s)::is, m⟩ []) = stack.result r) :=
+
+theorem call_trace {pc: program α} {s: source α} {p is: program α} {m m' mr r: memory α} {n: ℕ} {cs: list (program α × memory α)} {rs: list (memory α)}:
+  m.getms s = m' →
+  pc.has_result m' mr →
+  thunk.has_trace ⟨p, is, m.setm 0 mr⟩ ⟨r, n, cs, rs⟩ →
+  thunk.has_trace ⟨p, (instruction.call pc s)::is, m⟩ ⟨r, n+1, (pc,m')::cs, rs⟩ :=
+begin
+  intros hm hres htr,
+  apply step_trace _ _ htr,
+  { simpa only [thunk.step_over, thunk.step,
+      option.get_or_else, option.map_none',
+      hm, memory.getm_setm, memory.setm_setm, thunk.set_result,
+      eq_self_iff_true, and_true] using hres },
+  { unfold thunk.extend_trace thunk.step,
+    rw [hm] }
+end
+
+theorem recurse_trace {p: program α} {s: source α} {is: program α} {m m' mr r: memory α} {n: ℕ} {cs: list (program α × memory α)} {rs: list (memory α)}:
+  m.getms s = m' →
+  p.has_result m' mr →
+  thunk.has_trace ⟨p, is, m.setm 0 mr⟩ ⟨r, n, cs, rs⟩ →
+  thunk.has_trace ⟨p, (instruction.recurse s)::is, m⟩ ⟨r, n+1, cs, m'::rs⟩ :=
+begin
+  intros hm hres htr,
+  apply step_trace _ _ htr,
+  { simpa only [thunk.step_over, thunk.step,
+      option.get_or_else, option.map_none',
+      hm, memory.getm_setm, memory.setm_setm, thunk.set_result,
+      eq_self_iff_true, and_true] using hres },
+  { unfold thunk.extend_trace thunk.step,
+    rw [hm] }
+end
+
+theorem end_trace {p: program α} {m m': memory α}:
+  m = m' → thunk.has_trace ⟨p, [], m⟩ ⟨m', 0, [], []⟩ := λ h, h ▸ thunk.has_trace.result p m
+
+end hmem
